\SubProblem
{Ø¬}
{
\begin{equation*}
\begin{aligned}
    H(X)    &= -\sum_{x \in X} P(x) \log_2 {P(x)} \\ 
            &= \frac{1}{2}\log_2 2 + \frac{1}{4}\log_2 4 + \frac{1}{8}\log_2 8 + \frac{1}{8}\log_2 8 \\
            &= \frac{1}{2} + \frac{1}{2} + \frac{3}{8} + \frac{3}{8} = \frac{7}{4} [\frac{bits}{symbol}]
\end{aligned}
\end{equation*}
    
\begin{equation*}
\begin{aligned}
    H(Y)    &= -\sum_{y \in Y} P(y) \log_2 {P(y)} \\ 
            &= \frac{1}{4}\log_2 4 + \frac{1}{4}\log_2 4 + \frac{1}{4}\log_2 4 + \frac{1}{4}\log_2 4 \\
            &= \frac{1}{2} + \frac{1}{2} + \frac{1}{2} + \frac{1}{2} = 2 [\frac{bits}{symbol}]
\end{aligned}
\end{equation*}

\begin{equation*}
\begin{aligned}
    H(X,Y) &= -\sum_{x \in X}\sum_{y \in Y} P(x,y) \log_2 {P(x,y)} \\
    &= \frac{1}{8}\log_2 8 + \frac{1}{16}\log_2 16 + \frac{1}{32}\log_2 32 + \frac{1}{32}\log_2 32 + \frac{1}{16}\log_2 16 \\
    &+ \frac{1}{8}\log_2 8 + \frac{1}{32}\log_2 32 + \frac{1}{32}\log_2 32
    + \frac{1}{16}\log_2 16 + \frac{1}{16}\log_2 16 \\
    &+ \frac{1}{16}\log_2 16 + \frac{1}{16}\log_2 16 + \frac{1}{4}\log_2 4 + 0 + 0 + 0 \\
    &= \frac{3}{8} + \frac{1}{4} + \frac{5}{32} + \frac{5}{32}
    + \frac{1}{4} + \frac{3}{8} + \frac{5}{32} + \frac{5}{32} + \frac{1}{4} + \frac{1}{4} + \frac{1}{4} + \frac{1}{4} + \frac{1}{2} \\
    &= \frac{27}{8} [\frac{bits}{symbol}]
\end{aligned}
\end{equation*}
}