\SubProblem
{ل}
{
\begin{equation*}
\begin{aligned}
    H(Y) &= -\sum_{y \in Y} P(y) \log_2 {P(y)}\\
    &= \frac{1}{4}\log_2 4 + \frac{1}{4}\log_2 4 + \frac{1}{4}\log_2 4 + \frac{1}{4}\log_2 4 \\
    &= \frac{1}{2} + \frac{1}{2} + \frac{1}{2} + \frac{1}{2} = 2 [\frac{bits}{symbol}]
\end{aligned}
\end{equation*}

\begin{equation*}
\begin{aligned}
    H(X) &= -\sum_{x \in X} P(x) \log_2 {P(x)}\\
    &= \frac{1}{4}\log_2 4 + \frac{1}{4}\log_2 4 + \frac{1}{4}\log_2 4 + \frac{1}{4}\log_2 4 \\
    &= \frac{1}{2} + \frac{1}{2} + \frac{1}{2} + \frac{1}{2} = 2 [\frac{bits}{symbol}]
\end{aligned}
\end{equation*}
    
\begin{equation*}
\begin{aligned}
    H(X,Y) &= -\sum_{x \in X}\sum_{y \in Y} P(x,y) \log_2 {P(x,y)}\\
    &= 16(\frac{1}{16}\log_2 16) \\
    &= 16 \times \frac{1}{4} = 4 [\frac{bits}{symbol}]
\end{aligned}
\end{equation*}

    مقادیر 
    \lr{$H(X)$}
    و
    \lr{H(X,Y)}
    نسبت به قسمت (ج) بیشتر شده است اما مقدار
    \lr{$H(Y)$}
    تغییری نکرده است.
}